done refactoring

src/example/TemporalLogicFull.v
@@ -6,6 +6,14 @@ From stdpp Require Export coPset gmap namespaces.
 From Fairness Require Import SCMem.
 Require Import Program.
 
+(** User-defined auxiliary atoms. *)
+
+Section AUXRAS.
+
+  Definition ExclUnitsRA : URA.t := (nat ==> (Excl.t unit))%ra.
+  Definition AuthExclRA (A : Type) : URA.t := (Auth.t (Excl.t A)).
+
+End AUXRAS.
 
 Section XADEF.
 
@@ -28,20 +36,36 @@ End XADEF.
 
 Section AUXRAS.
 
-  Definition ExclUnitsRA : URA.t := (nat ==> (Excl.t unit))%ra.
-  Definition AuthExclRA (A : Type) : URA.t := (Auth.t (Excl.t A)).
+  Class AUXRAs (Σ : GRA.t) :=
+    {
+      (* SCMem related RAs *)
+      _MEMRA: @GRA.inG memRA Σ;
+      (* Map from nat to Excl unit RA. *)
+      _EXCLUNITS: @GRA.inG ExclUnitsRA Σ;
+      (* Auth Excl Qp RA. *)
+      _AUEX_QP: @GRA.inG (AuthExclRA Qp) Σ;
+    }.
 
 End AUXRAS.
+
+Section EXPORT.
+
+  Context `{Σ : GRA.t}.
+  Context {AUXRAS : AUXRAs Σ}.
+
+  (* SCMem related RAs *)
+  #[export] Instance MEMRA: @GRA.inG memRA Σ:= _MEMRA.
+  (* Map from nat to Excl unit RA. *)
+  #[export] Instance EXCLUNITS: @GRA.inG ExclUnitsRA Σ:= _EXCLUNITS.
+  (* Auth Excl Qp RA. *)
+  #[export] Instance AUEX_QP: @GRA.inG (AuthExclRA Qp) Σ:= _AUEX_QP.
+
+End EXPORT.
 
 Section XAINTERP.
 
   Context `{Σ : GRA.t}.
-  (* SCMem related RAs. *)
-  Context `{MEMRA: @GRA.inG memRA Σ}.
-  (* Map from nat to Excl unit RA. *)
-  Context `{EXCLUNITS: @GRA.inG ExclUnitsRA Σ}.
-  (* Auth Excl Qp RA. *)
-  Context `{AUEX_QP: @GRA.inG (AuthExclRA Qp) Σ}.
+  Context {AUXRAS : AUXRAs Σ}.
 
   Definition xatom_sem (xa : xatom) : iProp :=
     match xa with
@@ -59,97 +83,18 @@ Section XAINTERP.
 End XAINTERP.
 
 (** Notations. *)
-Notation "'➢' s" := (⟨Atom.aux (AA:=XAtom) s⟩)%F (at level 90) : formula_scope.
+Notation "'➢' s" := (⟨Atom.aux (AA:=XAtom) s⟩)%F (at level 50) : formula_scope.
 Notation "l ↦ v" := (➢ (scm_points_to l v))%F (at level 90) : formula_scope.
 
-Section TLRAS.
 
-  Class TLRAs (STT : StateTypes) (Σ : GRA.t) :=
-    {
-      (* Invariant related default RAs *)
-      _OWNESRA : @GRA.inG OwnEsRA Σ;
-      _OWNDSRA : @GRA.inG OwnDsRA Σ;
-      _IINVSETRA : @GRA.inG (IInvSetRA (@Formula XAtom STT)) Σ;
-      (* State related default RAs *)
-      _THDRA: @GRA.inG ThreadRA Σ;
-      _STATESRC: @GRA.inG (stateSrcRA st_src_type) Σ;
-      _STATETGT: @GRA.inG (stateTgtRA st_tgt_type) Σ;
-      _IDENTSRC: @GRA.inG (identSrcRA id_src_type) Σ;
-      _IDENTTGT: @GRA.inG (identTgtRA id_tgt_type) Σ;
-      (* Liveness logic related default RAs *)
-      _OBLGRA: @GRA.inG ObligationRA.t Σ;
-      _EDGERA: @GRA.inG EdgeRA Σ;
-      _ARROWSHOTRA: @GRA.inG ArrowShotRA Σ;
-      _ARROWRA: @GRA.inG (@ArrowRA id_tgt_type Formula) Σ;
-      (* SCMem related RAs *)
-      _MEMRA: @GRA.inG memRA Σ;
-      (* Map from nat to Excl unit RA. *)
-      _EXCLUNITS: @GRA.inG ExclUnitsRA Σ;
-      (* Auth Excl Qp RA. *)
-      _AUEX_QP: @GRA.inG (AuthExclRA Qp) Σ;
-    }.
-
-End TLRAS.
-
-Section EXPORT.
-
-  Context {STT : StateTypes}.
-  Context `{Σ : GRA.t}.
-  Context {TLRAS : TLRAs STT Σ}.
-
-  (* Invariant related default RAs *)
-  #[export] Instance OWNESRA : @GRA.inG OwnEsRA Σ := _OWNESRA.
-  #[export] Instance OWNDSRA : @GRA.inG OwnDsRA Σ:= _OWNDSRA.
-  #[export] Instance IINVSETRA : @GRA.inG (IInvSetRA Formula) Σ:= _IINVSETRA.
-  (* State related default RAs *)
-  #[export] Instance THDRA: @GRA.inG ThreadRA Σ:= _THDRA.
-  #[export] Instance STATESRC: @GRA.inG (stateSrcRA st_src_type) Σ:= _STATESRC.
-  #[export] Instance STATETGT: @GRA.inG (stateTgtRA st_tgt_type) Σ:= _STATETGT.
-  #[export] Instance IDENTSRC: @GRA.inG (identSrcRA id_src_type) Σ:= _IDENTSRC.
-  #[export] Instance IDENTTGT: @GRA.inG (identTgtRA id_tgt_type) Σ:= _IDENTTGT.
-  (* Liveness logic related default RAs *)
-  #[export] Instance OBLGRA: @GRA.inG ObligationRA.t Σ:= _OBLGRA.
-  #[export] Instance EDGERA: @GRA.inG EdgeRA Σ:= _EDGERA.
-  #[export] Instance ARROWSHOTRA: @GRA.inG ArrowShotRA Σ:= _ARROWSHOTRA.
-  #[export] Instance ARROWRA: @GRA.inG (@ArrowRA id_tgt_type Formula) Σ:= _ARROWRA.
-  (* SCMem related RAs *)
-  #[export] Instance MEMRA: @GRA.inG memRA Σ:= _MEMRA.
-  (* Map from nat to Excl unit RA. *)
-  #[export] Instance EXCLUNITS: @GRA.inG ExclUnitsRA Σ:= _EXCLUNITS.
-  (* Auth Excl Qp RA. *)
-  #[export] Instance AUEX_QP: @GRA.inG (AuthExclRA Qp) Σ:= _AUEX_QP.
-
-End EXPORT.
-
-Section TL.
+Section TLFULL.
 
   Context {STT : StateTypes}.
 
   Context `{Σ : GRA.t}.
-  (* (* Invariant related default RAs *) *)
-  (* Context `{OWNESRA : @GRA.inG OwnEsRA Σ}. *)
-  (* Context `{OWNDSRA : @GRA.inG OwnDsRA Σ}. *)
-  (* Context `{IINVSETRA : @GRA.inG (IInvSetRA Formula) Σ}. *)
-  (* (* State related default RAs *) *)
-  (* Context `{THDRA: @GRA.inG ThreadRA Σ}. *)
-  (* Context `{STATESRC: @GRA.inG (stateSrcRA st_src_type) Σ}. *)
-  (* Context `{STATETGT: @GRA.inG (stateTgtRA st_tgt_type) Σ}. *)
-  (* Context `{IDENTSRC: @GRA.inG (identSrcRA id_src_type) Σ}. *)
-  (* Context `{IDENTTGT: @GRA.inG (identTgtRA id_tgt_type) Σ}. *)
-  (* (* Liveness logic related default RAs *) *)
-  (* Context `{OBLGRA: @GRA.inG ObligationRA.t Σ}. *)
-  (* Context `{EDGERA: @GRA.inG EdgeRA Σ}. *)
-  (* Context `{ONESHOTRA: @GRA.inG ArrowShotRA Σ}. *)
-  (* Context `{ARROWRA: @GRA.inG (@ArrowRA id_tgt_type Formula) Σ}. *)
-  (* (* SCMem related RAs *) *)
-  (* Context `{MEMRA: @GRA.inG memRA Σ}. *)
-  (* (* Map from nat to Excl unit RA. *) *)
-  (* Context `{EXCLUNITS: @GRA.inG ExclUnitsRA Σ}. *)
-  (* (* Auth Excl Qp RA. *) *)
-  (* Context `{AUEX_QP: @GRA.inG (AuthExclRA Qp) Σ}. *)
-
-  Context {TLRAS : TLRAs STT Σ}.
+  Context {TLRAS : @TLRAs XAtom STT Σ}.
+  Context {AUXRAS : AUXRAs Σ}.
 
   Global Instance TLSet : @IInvSet Σ (@Formula XAtom STT) := SynIISet.
 
-End TL.
+End TLFULL.
